many changes

theories/Atom.v
@@ -5,82 +5,95 @@ From mathcomp.ssreflect Require Import ssreflect ssrbool ssrnat ssrfun eqtype se
 Require Import FinMap.ordtype.
 
 Require Import Omega.
+Require Import Coq.Structures.Equalities.
 
+ Require Import Lia.
+Require Import PP.Ppsimplmathcomp. 
+(* Require Import Coq.Arith.Max.
+Require Metalib.Metatheory.*)
+Require Coq.Lists.List.
+Require Import Metalib.CoqListFacts.
+Require Metalib.LibTactics.
+
+
+(* Require Import Metalib.LibTactics. *)
+
+(* Require Import Structures.Orders. *)
+(*Notation In := Lists.List.In.*)
 Set Implicit Arguments.
 Unset Strict Implicit.
 Import Prenex Implicits.
 
-Module Type ATOM.
 
-  Parameter atom : Set.
-  Definition t := atom.
+Require Import FSets.
 
-  (* atoms can be compared to booleans *)
+Require Import Structures.OrderedType.
+Print Nat_as_OT.
 
-  Parameter eq_atom : atom -> atom -> bool.
-  Parameter eq_reflect : forall (a b : atom), ssrbool.reflect (a = b) (eq_atom a b).
-  Parameter atom_eqMixin : Equality.mixin_of atom.
-  Canonical atom_eqType := EqType atom atom_eqMixin.
+Locate In. 
+
+Require Import SendRec.MapFunction.
 
 
-  (* atoms can be ordered with an irreflexive order *)
-
-  Parameter ltn : atom -> atom -> bool.
-  Parameter ltn_irreflexive : forall x : atom, ltn x x = false.
-  Parameter ltn_transitive : forall y x z : atom,
-      ltn x y -> ltn y z -> ltn x z.
-  Parameter ltn_total : forall a b : atom, [|| ltn a b, eq_atom a b | ltn b a].
-  Parameter atom_ordMixin : Ordered.mixin_of atom_eqType.
-  Canonical atom_ordType := OrdType atom atom_ordMixin.
-
-  Parameter fresh : seq atom -> atom.
-
-  Parameter fresh_not_in : forall l, (fresh l) \notin l.
-
-  Parameter nat_of : atom -> nat.
-End ATOM.
-
-Module Atom : ATOM.
-
-  (* begin hide *)
-  Definition atom := nat.
-  Definition t := atom.
-
-  Definition eq_atom (a b : nat) : bool := ssrnat.eqn a b.
-
-  Lemma eq_reflect a b :  ssrbool.reflect (a = b) (eq_atom a b).
+Module Atom <: OrderedType.
+ Include Nat_as_OT. Print Nat_as_OT.
+ Definition eq_atom (a b : t) : bool := ssrnat.eqn a b.  
+ Lemma eq_reflect a b :  ssrbool.reflect (a = b) (eq_atom a b).
   Proof. by apply: ssrnat.eqnP. Qed.
 
+
+  Lemma eq_atom_refl : forall (a : t), eq_atom a a.
+  Proof. Search "nat_refl". Check ssrnat.eqnP. rewrite /eq_atom. elim. done. done. 
+  Qed.
+
+  Scheme Equality for nat.
+  
+  Lemma eq_atom_neq : forall a b, a<> b -> eq_atom a b = false.
+  Proof. move => a b /eqP. case (eq_reflect a b).  move => H /eqP. done. done.  Qed. 
+
   Definition atom_eqMixin := EqMixin Atom.eq_reflect.
-  Canonical atom_eqType := EqType atom atom_eqMixin.
+  Canonical atom_eqType := EqType t atom_eqMixin.
 
-  (* equality and ordered *)
-
-  Definition ltn a b := a  < b.
-  Lemma ltn_irreflexive : forall x : nat, x < x = false.
+ Lemma max_lt_r : forall x y z,
+    x <= z -> x <= max y z.
   Proof.
-    intros ; apply ssrnat.ltnn.
+    induction x. auto with arith.
+    induction y. auto with arith.
+      simpl. induction z; ppsimpl;lia. 
   Qed.
 
-  Definition ltn_transitive := ssrnat.ltn_trans.
 
-  Lemma ltn_total : forall a b : nat, [|| a < b, a == b | b < a].
+ Lemma nat_list_max : forall (xs : list nat),
+    { n : nat | forall x, In x xs -> x <= n }.
   Proof.
-    move=> a b.
-    rewrite/lt/eq.
-    case ssrnat.ltngtP ; move=>H ; intuition ; rewrite Bool.orb_comm ; intuition.
+   induction xs as [ | x xs [y H] ].
+    (* case: nil *)
+    exists 0. inversion 1.
+    (* case: cons x xs *)
+    exists (max x y). intros z J. simpl in J. destruct J as [K | K].
+    - subst. ppsimpl. lia.  auto using max_lt_r. 
+Qed.
+
+  Lemma atom_fresh_for_list :
+    forall (xs : list nat), { n : nat | ~ In n xs }.
+  Proof.
+   intros xs. destruct (nat_list_max xs) as [x H].
+    exists (S x). intros J. lapply (H (S x)). ppsimpl. lia. trivial.
   Qed.
 
-  Definition atom_ordMixin : Ordered.mixin_of atom_eqType :=
-    @OrdMixin
-      atom_eqType
-      ltn
-      ltn_irreflexive
-      ltn_trans
-      ltn_total.
-  Canonical atom_ordType := OrdType atom atom_ordMixin.
+Check exist.
+  Definition fresh (l : list t) :=
+    match atom_fresh_for_list l with
+      (exist x _) => x
+    end.
 
-  Fixpoint fresh' a (l : seq atom) :=
+  Lemma fresh_not_in : forall l, ~ In (fresh l)  l.
+  Proof.
+    intro l. unfold fresh.
+    destruct atom_fresh_for_list. auto.
+  Qed.
+
+ (* Fixpoint fresh' a (l : seq atom) :=
     match l with
     | [::] => a +1
     | x::xs => fresh' (maxn x a) xs
@@ -100,18 +113,187 @@ Module Atom : ATOM.
     suff fresh'_not_in a : fresh' a l \notin l by apply fresh'_not_in.
     elim: l a =>  // a' l IHl a.
       by rewrite /fresh/fresh' in_cons Bool.negb_orb fresh_not_head ?(IHl (maxn a' a)) ?leq_maxl.
-  Qed.
+  Qed.*)
 
-  Definition nat_of (x : atom) := x.
+  Definition nat_of (x : t) := x.
   (* end hide *)
+
 End Atom.
 
-(** We make [atom], [fresh], [fresh_not_in] and [atom_fresh_for_list] available
-    without qualification. *)
+Definition nat_beq := Atom.nat_beq.
+Definition nat_eq_dec := Atom.nat_eq_dec.
 
-Notation atom := Atom.atom.
+Canonical atom_eqType := EqType Atom.t Atom.atom_eqMixin.
+
+Module M := FSetAVL.Make(Atom).
+
+Module MapFunction := MapFunction M.
+
+Locate In.
+
+Notation atom := Atom.t. 
+Notation atoms := M.t.
 Notation fresh := Atom.fresh.
 Notation fresh_not_in := Atom.fresh_not_in.
+Notation atom_fresh_for_list := Atom.atom_fresh_for_list.
 
-Canonical atom_eqType := EqType Atom.atom Atom.atom_eqMixin.
-Canonical atom_ordType := OrdType Atom.atom Atom.atom_ordMixin.
+
+(** The [AtomSetDecide] module provides the [fsetdec] tactic for
+    solving facts about finite sets of atoms. *)
+
+Module Export AtomSetDecide := Coq.FSets.FSetDecide.WDecide_fun Atom M.
+
+(** The [AtomSetNotin] module provides the [destruct_notin] and
+    [solve_notin] for reasoning about non-membership in finite sets of
+    atoms, as well as a variety of lemmas about non-membership. *)
+
+(* Module Export AtomSetNotin := FSetWeakNotin.Notin_fun Atom AtomSetImpl. *)
+
+(** Given the [fsetdec] tactic, we typically do not need to refer to
+    specific lemmas about finite sets.  However, instantiating
+    functors from the FSets library makes a number of setoid rewrites
+    available.  These rewrites are crucial to developments since they
+    allow us to replace a set with an extensionally equal set (see the
+    [Equal] relation on finite sets) in propositions about finite
+    sets. *)
+
+Module MF := FSetFacts.Facts M.
+
+Module MP := FSetProperties.Properties M.
+
+
+Export MF.
+
+Export MP.
+(* ********************************************************************** *)
+(** * Properties *)
+
+(** For any given finite set of atoms, we can generate an atom fresh
+    for it. *)
+(*
+Lemma test : forall (l : seq atom) a ,a \in (elements l) <-> In a l.
+Proof.
+move=> l.
+elim : elements l. - move => l a. H. 
+*)
+
+
+
+
+Lemma atom_fresh : forall L : atoms, { x : atom | ~ M.In x L }.
+Proof.
+  intros L. destruct (atom_fresh_for_list (M.elements L)) as [a H].
+  exists a. intros J. contradiction H. Search "InA".  Search "InA_iff_In". Search _ (M.elements _). Print InA.  Search "In_InA". 
+  rewrite <- CoqListFacts.InA_iff_In. auto using M.elements_1.
+Qed.
+
+
+
+(* ********************************************************************** *)
+(** * Tactic support for picking fresh atoms *)
+
+(* begin hide *)
+
+(** The auxiliary tactic [simplify_list_of_atom_sets] takes a list of
+    finite sets of atoms and unions everything together, returning the
+    resulting single finite set. *)
+
+Locate empty.
+Locate Ltac ltac_remove_dups. 
+Ltac simplify_list_of_atom_sets L :=
+  let L := eval simpl in L in
+  let L := LibTactics.ltac_remove_dups L in
+  let L := eval simpl in (List.fold_right M.union M.empty L) in
+  match L with
+    | context C [M.union ?E M.empty] => context C [ E ]
+  end.
+
+(* end hide *)
+
+(** [gather_atoms_with F] returns the union of all the finite sets
+    [F x] where [x] is a variable from the context such that [F x]
+    type checks. *)
+
+Ltac gather_atoms_with F :=
+  let apply_arg x :=
+    match type of F with
+      | _ -> _ -> _ -> _ => constr:(@F _ _ x)
+      | _ -> _ -> _ => constr:(@F _ x)
+      | _ -> _ => constr:(@F x)
+    end in
+  let rec gather V :=
+    match goal with
+      | H : _ |- _ =>
+        let FH := apply_arg H in
+        match V with
+          | context [FH] => fail 1
+          | _ => gather (M.union FH V)
+        end
+      | _ => V
+    end in
+  let L := gather M.empty in eval simpl in L.
+
+(** [beautify_fset V] assumes that [V] is built as a union of finite
+    sets and returns the same set cleaned up: empty sets are removed
+    and items are laid out in a nicely parenthesized way. *)
+
+Ltac beautify_fset V :=
+  let rec go Acc E :=
+     match E with
+     | M.union ?E1 ?E2 => let Acc2 := go Acc E2 in go Acc2 E1
+     | M.empty => Acc
+     | ?E1 => match Acc with
+                | M.empty => E1
+                | _ => constr:(M.union E1 Acc)
+              end
+     end
+  in go M.empty V.
+
+(** The tactic [pick fresh Y for L] takes a finite set of atoms [L]
+    and a fresh name [Y], and adds to the context an atom with name
+    [Y] and a proof that [~ In Y L], i.e., that [Y] is fresh for [L].
+    The tactic will fail if [Y] is already declared in the context.
+    The variant [pick fresh Y] is similar, except that [Y] is fresh
+    for "all atoms in the context."  This version depends on the
+    tactic [gather_atoms], which is responsible for returning the set
+    of "all atoms in the context."  By default, it returns the empty
+    set, but users are free (and expected) to redefine it. *)
+
+Ltac gather_atoms :=
+  constr:(M.empty).
+
+Tactic Notation "pick" "fresh" ident(Y) "for" constr(L) :=
+  let Fr := fresh "Fr" in
+  let L := beautify_fset L in
+  (destruct (atom_fresh L) as [Y Fr]).
+
+Tactic Notation "pick" "fresh" ident(Y) :=
+  let L := gather_atoms in
+  pick fresh Y for L.
+
+Ltac pick_fresh y :=
+  pick fresh y.
+
+(** Example: We can redefine [gather_atoms] to return all the
+    "obvious" atoms in the context using the [gather_atoms_with] thus
+    giving us a "useful" version of the "[pick fresh]" tactic. *)
+
+Ltac gather_atoms ::=
+  let A := gather_atoms_with (fun x : atoms => x) in
+  let B := gather_atoms_with (fun x : atom => M.singleton x) in
+  constr:(M.union A B).
+
+Lemma example_pick_fresh_use : forall (x y z : atom) (L1 L2 L3: atoms), True.
+(* begin show *)
+Proof.
+  intros x y z L1 L2 L3.
+  pick fresh k.
+
+  (** At this point in the proof, we have a new atom [k] and a
+      hypothesis [Fr] that [k] is fresh for [x], [y], [z], [L1], [L2],
+      and [L3]. *)
+
+  trivial.
+Qed.
+(* end show *)
+
