theories/Nom_SyntaxBST.v
@@ -11,110 +11,15 @@ Require Import PP.Ppsimplmathcomp.
 Require Import Equations.Equations.
 Require Import SendRec.Atom.
 
-Inductive sort : Set :=
-  | boole : sort (* boolean expression *)
-  | end_points : tp -> tp -> sort
-with tp : Set :=
-  | input : sort -> tp -> tp
-  | output : sort -> tp -> tp
-  | ch_input : tp -> tp -> tp
-  | ch_output : tp -> tp -> tp
-  | offer_branch : tp -> tp -> tp
-  | take_branch : tp -> tp -> tp
-  | ended : tp
-  | bot : tp
-.
 
-Scheme tp_sort := Induction for tp Sort Prop
-  with sort_tp := Induction for sort Sort Prop. (* Minimality *)
-Combined Scheme tp_sort_mutind from tp_sort, sort_tp.
+Notation "E `union` F" :=
+  (M.union E F)
+  (at level 65, right associativity, format "E  `union`  '/' F").
 
-Fixpoint dual (T : tp) : tp :=
-  match T with
-  | input s T => output s (dual T)
-  | output s T => input s (dual T)
-  | ch_input T T' => ch_output T (dual T')
-  | ch_output T T' => ch_input T (dual T')
-  | offer_branch T T' => take_branch (dual T) (dual T')
-  | take_branch T T' => offer_branch (dual T) (dual T')
-  | ended => ended
-  | bot => bot
-  end
-.
-
-Lemma dual_is_dual t : dual (dual t) = t.
-  elim t=>// ; rewrite/dual ; move=>//; rewrite-/dual ;
-    do ? (move=> s t0 =>->) ;
-    do ? (move=> t0 R' t1 =>->) ;
-    rewrite ?R' ;
-   easy.
-Qed.
-
-Lemma double_dual t: t = dual(dual t).
-Proof.
-  elim t=>//; rewrite/dual=>//; rewrite-/dual ; congruence.
-Qed.
-
-Fixpoint eq_tp (T T': tp) : bool :=
-  match T, T' with
-  | input s T, input s' T' => eq_sort s s' && eq_tp T T'
-  | output s T, output s' T' => eq_sort s s' && eq_tp T T'
-  | ch_input T1 T2, ch_input T1' T2' => eq_tp T1 T1' && eq_tp T2 T2'
-  | ch_output T1 T2, ch_output T1' T2' => eq_tp T1 T1' && eq_tp T2 T2'
-
-  | offer_branch T1 T2, offer_branch T1' T2' => eq_tp T1 T1' && eq_tp T2 T2'
-  | take_branch T1 T2, take_branch T1' T2' => eq_tp T1 T1' && eq_tp T2 T2'
-  | ended, ended => true
-  | bot, bot => true
-  | _, _ => false
-  end
-with eq_sort (s s' : sort) : bool :=
-  match s, s' with
-  | boole, boole => true
-  | end_points T1 T2, end_points T1' T2' => eq_tp T1 T1' && eq_tp T2 T2'
-  | _, _ => false
-  end.
-
-Lemma eq_imp_eq : (forall x y, eq_tp x y -> x = y) /\ forall s s', eq_sort s s' -> s = s'.
-Proof.
-  apply tp_sort_mutind ; intros; try destruct y  ; try destruct s'; try easy ;
-  inversion H1 ; apply Bool.andb_true_iff in H3 ; destruct H3 ;
-  try(move:H3 ; move/H0=>H3 ; move:H2 ; move/H=>H4 ; by rewrite H3 H4).
-Qed.
-
-Lemma eq_tp_refl x : eq_tp x x.
-Proof.
-  by elim x using tp_sort with (P:=fun x=>eq_tp x x) (P0:= fun s=>eq_sort s s)=>//;
-     move=>s H t H0; simpl; rewrite H H0.
-Qed.
-
-Lemma eq_sort_refl s : eq_sort s s.
-Proof.
-  by elim s using sort_tp with (P:=fun x=> eq_tp x x)=>//;
-     move=>x H t H0; simpl; rewrite H H0.
-Qed.
-
-Lemma eq_tpP : Equality.axiom eq_tp.
-Proof.
-  move=>x y.
-  apply: (iffP idP)=>[|<-].
-  apply eq_imp_eq.
-  apply eq_tp_refl.
-Qed.
-
-Lemma eq_sortP : Equality.axiom eq_sort.
-Proof.
-  move=>x y.
-  apply: (iffP idP)=>[|<-].
-  apply eq_imp_eq.
-  apply eq_sort_refl.
-Qed.
-
-Canonical tp_eqMixin := EqMixin eq_tpP.
-Canonical tp_eqType := Eval hnf in EqType tp tp_eqMixin.
-
-Canonical sort_eqMixin := EqMixin eq_sortP.
-Canonical sort_eqType := Eval hnf in EqType sort sort_eqMixin.
+Notation singleton := M.singleton.
+Notation remove := M.remove.
+Notation add := M.add.
+Notation empty := M.empty.
 
 Inductive exp : Set :=
   | tt
@@ -122,15 +27,30 @@ Inductive exp : Set :=
   | var : atom -> exp
 .
 
-Definition eq_atom := Atom.eq_atom.
 Definition exp_eqb e0 e1 : bool :=
 match (e0,e1) with
 | (tt,tt) => true
 | (ff,ff) => true
-| (var nm0,var nm1) => eq_atom nm0 nm1
+| (var nm0,var nm1) => nm0 == nm1
 | _ => false
 end.
 
+Lemma exp_eqb_reflect : forall a b, ssrbool.reflect (a = b) (exp_eqb a b).
+Proof.
+elim. 
+- elim; rewrite /exp_eqb; try ((constructor + constructor 2);done). 
+- elim; rewrite /exp_eqb; try ((constructor + constructor 2);done). 
+- move => t. elim. 
+ *  rewrite /exp_eqb; try ((constructor + constructor 2);done). 
+ *  rewrite /exp_eqb; try ((constructor + constructor 2);done). 
+ * move => t1. rewrite /exp_eqb. case : (Atom.eq_reflect t t1).
+  ** move=>->. rewrite eq_refl. constructor. done. 
+  **  move => x; have copy := x; move: copy x. rewrite /eq_op.   rewrite /=. move/ Atom.eq_atom_neq=>->. constructor. intro H.  inversion H. done. 
+Qed.
+
+
+Definition exp_eqMixin := EqMixin exp_eqb_reflect.
+Canonical atom_eqType := EqType exp exp_eqMixin.
 
 Inductive proc : Set :=
 | send : atom -> exp -> proc -> proc
@@ -145,50 +65,65 @@ Inductive proc : Set :=
 | nu_ch : atom -> proc -> proc
 .
 
+
 Notation "k ![ e ] ; p0" := (send k e p0)(at level 70) .
 Notation "k ? ( x ) 'in' p0" := (receive k x p0)(at level 70) .
-
-
 Notation "p0 |||| p1" := (par p0 p1)(at level 81, left associativity) .
 
 Fixpoint proc_eqb p0 p1 := 
 match p0,p1 with
-| (send a0 e0 p0'),(send a1 e1 p1') => eq_atom a0 a1 && exp_eqb e0 e1 && proc_eqb p0' p1'
-| (receive a0 a0' p0'),(receive a1 a1' p1') => eq_atom a0 a1 && eq_atom a0' a1' && proc_eqb p0' p1'
-| (throw a0 a0' p0'),(throw a1 a1' p1') => eq_atom a0 a1 && eq_atom a0' a1' && proc_eqb p0' p1'
-| (catch a0 a0' p0'),(catch a1 a1' p1') => eq_atom a0 a1 && eq_atom a0' a1' && proc_eqb p0' p1'
+| (send a0 e0 p0'),(send a1 e1 p1') => (a0 == a1) && (e0 == e1) && proc_eqb p0' p1'
+| (receive a0 a0' p0'),(receive a1 a1' p1') => (a0 == a1) && (a0' == a1') && proc_eqb p0' p1'
+| (throw a0 a0' p0'),(throw a1 a1' p1') => (a0 == a1) && (a0' == a1') && proc_eqb p0' p1'
+| (catch a0 a0' p0'),(catch a1 a1' p1') => (a0 == a1) && (a0' == a1') && proc_eqb p0' p1'
 | (par p0' p0''),(par p1' p1'') => proc_eqb p0' p1' && proc_eqb p0'' p1''
 | inact,inact => true
-| nu_ch nm0 p0', nu_ch nm1 p1' => eq_atom nm0 nm1 && proc_eqb p0' p1'
+| nu_ch nm0 p0', nu_ch nm1 p1' => (nm0 == nm1) && proc_eqb p0' p1'
 | _,_ => false 
-end.
+end. 
 
-Definition fv_exp (e : exp) : seq atom  :=
+(*add proc to the equality type class later*)
+
+
+Fixpoint fv_nm (P : proc) : atoms :=
+  match P with
+  | send nm e P0 => (singleton nm) `union` (fv_nm P0)
+  | receive nm0 nm1 P0 => (singleton nm0) `union` (fv_nm P0)
+  | throw nm0 nm1 P0 => ((singleton nm0) `union` (singleton nm1)) `union` (fv_nm P0) 
+  | catch nm0 nm1 P0 => (singleton nm0) `union` (remove nm1 (fv_nm P0))
+  | par P0 P1 => (fv_nm P0) `union` (fv_nm P1)
+  | inact => empty
+  | nu_ch nm P0 => remove nm (fv_nm P0)
+end.   
+
+
+Definition fv_exp_aux (e : exp) : atoms  :=
   match e with
-    | tt => [::]
-    | ff => [::]
-    | var a =>  [::a]
+    | tt => M.empty
+    | ff => M.empty
+    | var a =>  M.singleton a
   end.
 
-Fixpoint fv (P : proc) : seq atom :=
+
+Fixpoint fv_exp (P : proc) : atoms :=
   match P with
-  | send nm e P0 => [::nm] ++ (fv_exp e) ++ (fv P0)
-  | receive nm0 nm1 P0 => [::nm0] ++ (filter (predC1 nm1) (fv P0))
-  | throw nm0 nm1 P0 => [::nm0; nm1] ++ (fv P0) 
-  | catch nm0 nm1 P0 => [::nm0] ++ (filter (predC1 nm1) (fv P0))
-  | par P0 P1 => (fv P0) ++ (fv P1)
-  | inact => [::]
-  | nu_ch nm P0 => filter (predC1 nm) (fv P0)
+  | send nm e P0 => (fv_exp_aux e) `union` (fv_exp P0)
+  | receive nm0 nm1 P0 => remove nm1 (fv_exp P0)
+  | throw nm0 nm1 P0 => (fv_exp P0) 
+  | catch nm0 nm1 P0 => fv_exp P0
+  | par P0 P1 => (fv_exp P0) `union` (fv_exp P1)
+  | inact => empty
+  | nu_ch nm P0 => (fv_exp P0)
 end.          
 
 Definition swap_aux (b c a : atom) := 
   if (a == b) then c else if (a == c) then b else a.
 
           
-Fixpoint swap_exp (b c : atom) (e: exp) : exp :=
+Definition swap_exp (b c : atom) (e: exp)  : exp :=
   match e with
   | var nm => var (swap_aux b c nm)
-  | t => t
+  | _ => e
   end.
 
 Fixpoint swap (b c: atom) (P : proc) : proc :=
@@ -201,55 +136,111 @@ Fixpoint swap (b c: atom) (P : proc) : proc :=
   | inact => inact
   | nu_ch nm P0 => nu_ch (swap_aux b c nm) (swap b c P0)
   end.
-Print mem. Locate mem. Check mem_seq.
-Definition binder_eq f (p0 p1 : (atom * proc)) : bool :=
+
+
+Definition binder_eq_nm f (p0 p1 : (atom * proc)) : bool :=
 let (nm0,P0) := p0 in let (nm1,P1) := p1 in
-if eq_atom nm0 nm1 then f P0 P1
-                               else if mem_seq (fv P1) nm0 then false 
+if (nm0 == nm1) then f P0 P1
+                               else if M.mem nm0 (fv_nm P1) then false 
+                               else f P0 (swap nm0 nm1 P1).
+
+Definition binder_eq_exp f (p0 p1 : (atom * proc)) : bool :=
+let (nm0,P0) := p0 in let (nm1,P1) := p1 in
+if (nm0 == nm1) then f P0 P1
+                               else if M.mem nm0 (fv_exp P1) then false 
                                else f P0 (swap nm0 nm1 P1).
 
 
-Fixpoint aeq (P0 P1 : proc) : bool :=
-let binder_eq := binder_eq aeq in
+Fixpoint aeq (P0 P1 : proc) {struct P0} : bool :=
+let binder_eq_nm := binder_eq_nm aeq in
+let binder_eq_exp := binder_eq_exp aeq in
+
 match P0,P1 with
-| (send nm0 e0 P0'), (send nm1 e1 P1') => (eq_atom nm0 nm1) && (exp_eqb e0 e1) && (aeq P0' P1')
-| (receive nm0 nmb0 P0'), (receive nm1 nmb1 P1') => (eq_atom nm0 nm1) && (binder_eq (nmb0, P0') (nmb1, P1'))
-| (throw nm0 nm0' P0'), (throw nm1 nm1' P1') => (eq_atom nm0 nm1) && (eq_atom nm0' nm1') && (aeq P0' P1')
-| (catch nm0 nmb0 P0'), (receive nm1 nmb1 P1') => (eq_atom nm0 nm1) && (binder_eq (nmb0, P0') (nmb1, P1'))
-| (nu_ch nm0 P0), (nu_ch nm1 P1) => binder_eq (nm0, P0) (nm1, P1)
+| (send nm0 e0 P0'), (send nm1 e1 P1') => (nm0 == nm1) && (e0 == e1) && (aeq P0' P1')
+| (receive nm0 nmb0 P0'), (receive nm1 nmb1 P1') => (nm0 == nm1) && (binder_eq_exp (nmb0, P0') (nmb1, P1'))
+| (throw nm0 nm0' P0'), (throw nm1 nm1' P1') => (nm0 == nm1) && (nm0' == nm1') && (aeq P0' P1')
+| (catch nm0 nmb0 P0'), (catch nm1 nmb1 P1') => (nm0 == nm1) && (binder_eq_nm (nmb0, P0') (nmb1, P1'))
+| (nu_ch nm0 P0), (nu_ch nm1 P1) => binder_eq_nm (nm0, P0) (nm1, P1)
+| (par P0' P0''),(par P1' P1'') => (aeq P0' P1') && (aeq P0'' P1'')
+| inact, inact => true
 | _, _ => false
 end.
+
+Notation "P =A= Q" := (aeq P Q)(at level 70). 
 
 
 Reserved Notation "P === Q" (at level 70).
 Inductive congruent : proc -> proc -> Prop :=
 | c_refl P : P === P
-| c_alpha P Q (H: aeq P Q): P === P 
+| c_alpha P Q (H: aeq P Q): P === Q 
 | c_inact P : (par inact P) === P
 | c_comm P Q: (par P Q) === (par Q P)
 | c_asoc P Q R: (par (par P Q) R) === (par P (par Q R))
-| c_nu_ch P Q nm (H: nm \notin (fv Q)) : (par (nu_ch nm P) Q) === (nu_ch nm (par P Q))
+| c_nu_ch P Q nm (H: ~ M.In nm (fv_nm Q)) : (par (nu_ch nm P) Q) === (nu_ch nm (par P Q))
 | c_nu_ch_inact nm : nu_ch nm inact === inact
 where "P === Q" := (congruent P Q).
 
+(*broken, can capture variables*)
+Fixpoint swap_weak (b c: atom) (P : proc) : proc :=
+  match P with
+  | send nm e P0 => send nm e (swap_weak b c P0)
+  | receive nm0 nm1 P0 => receive nm0 (swap_aux b c nm1) (swap_weak b c P0)
+  | throw nm0 nm1 P0 => throw nm0 nm1 (swap_weak b c P0)
+  | catch nm0 nm1 P0 => catch nm0 (swap_aux b c nm1) (swap_weak b c P0)
+  | par P0 P1 => par (swap_weak b c P0) (swap_weak b c P1)
+  | inact => inact
+  | nu_ch nm P0 => nu_ch (swap_aux b c nm) (swap_weak b c P0)
+  end.
 
-Fixpoint congruent_fun P Q :=
-if proc_eqb P Q then true
-else if aeq P Q then true
-else match P, Q with
-     | (par inact P'),_ => proc_eqb P' Q
-     | (par (par P' P'') P'''),(par Q' (par Q'' Q''')) => proc_eqb P' Q' && proc_eqb P'' Q'' && proc_eqb P''' Q''' 
-     | (par P' P''),(par Q' Q'') => proc_eqb P' Q'' && proc_eqb P'' Q'
-     | (par (nu_ch nm P') P''), (nu_ch nm' (par Q' Q'')) => eq_atom nm nm' && proc_eqb P' Q' && proc_eqb P'' Q'' && (negb (mem_seq (fv P'') nm)) 
-     | (nu_ch m inact), inact => true 
-     | _, _ => false 
-     end.
+
+Ltac gather_atoms ::=
+  let A := gather_atoms_with (fun x : atoms => x) in
+  let B := gather_atoms_with (fun x : atom => M.singleton x) in
+  let C := gather_atoms_with (fun p : proc => fv_nm p) in
+
+  constr:(M.union A (M.union B C)).
+
+Definition alpha_variant (P : proc -> Prop) := forall p b c, P (swap_weak b c p) -> P p.
+
+Check proc_ind.
+Section PROC. 
+
+Variable Avoid : atoms.
+
+
+Variable  P : proc -> Prop.
+Hypothesis P_H : forall p b c, P (swap_weak b c p) <-> P p.
+Hypothesis (H :  (forall (t : atom) (e : exp) (p : proc), P p -> P (send t e p))).
+Hypothesis H1 :  (forall (t t0 : atom) (p : proc), ~ M.In t0 Avoid -> P p -> P (receive t t0 p)).
+Hypothesis H2 :  (forall (t t0 : atom) (p : proc), P p -> P (throw t t0 p)).
+Hypothesis H3 : (forall (t t0 : atom) (p : proc), ~ M.In t0 Avoid -> P p -> P (catch t t0 p)).
+Hypothesis H4 : (forall p : proc, P p -> forall p0 : proc, P p0 -> P (par p p0)).
+Hypothesis H5 : P inact.
+Hypothesis H6 : (forall (t : atom) (p : proc), P p -> P (nu_ch t p)).
+
+Lemma ind : forall p : proc, P p.
+Proof.  apply proc_ind.
+- apply H. 
+- move => t t0 p HP.  destruct (atom_fresh Avoid). apply (@P_H _ t0 x).  rewrite /=. 
+  rewrite /swap_aux eq_refl . apply H1. apply n. apply P_H. done. 
+- apply H2. 
+- move => t t0 p HP.  destruct (atom_fresh Avoid). apply (@P_H _ t0 x).  rewrite /=. 
+  rewrite /swap_aux eq_refl . apply H3. apply n. apply P_H. done. 
+- apply H4. 
+- apply H5. 
+- move => t p HP.  destruct (atom_fresh Avoid). apply (@P_H _ t x).  rewrite /=. 
+  rewrite /swap_aux eq_refl . apply H6. apply P_H. done. 
+Qed.
+
+End PROC.
+
+Check ind.
 
 
 
 Definition subst_exp (e : exp) (x : atom) (e_body : exp) : exp :=
   match e_body with
-  | var nm => if eq_atom nm x then e else var nm
+  | var nm => if nm == x then e else var nm
   | t => t
   end.
 
@@ -273,11 +264,20 @@ move => a0 p/= =>->//.
 Qed.
 
 Obligation Tactic := move => *;do ? ((do ? rewrite swap_size); apply : leP; rewrite /=; ppsimpl;lia).
+Check (fresh nil).
+Check (atom_fresh empty).  Check atom_fresh. 
+Check atom_fresh.
+Definition set_fresh (s :atoms) : atom := 
+  match atom_fresh s with
+  (exist x _) => x
+end. 
+
 
 Equations subst_proc_exp (e : exp) (x : atom) (P : proc) : proc by wf (proc_size P)  :=
 subst_proc_exp e x (send nm e0 P0) := send nm (subst_exp e x e0) (subst_proc_exp e x P0);
-subst_proc_exp e x (receive nm0 nm1 P0) := if eq_atom x nm1 then  (receive nm0 nm1 P0) 
-                                                        else receive nm0 (fresh (fv P0 ++ fv_exp e)) (subst_proc_exp e x (swap nm1 (fresh (fv P0 ++ fv_exp e)) P0));
+subst_proc_exp e x (receive nm0 nm1 P0) := if x == nm1 then  (receive nm0 nm1 P0) 
+                                           else receive nm0 (set_fresh (fv_exp P0 `union` fv_exp_aux e)) 
+                                                            (subst_proc_exp e x (swap nm1 (set_fresh (fv_exp P0 `union` fv_exp_aux e)) P0));
 subst_proc_exp e x (throw nm0 nm1 P0) := throw nm0 nm1 (subst_proc_exp e x P0);
 subst_proc_exp e x (catch nm0 nm1 P0) := catch nm0 nm1 (subst_proc_exp e x P0);
 subst_proc_exp e x (par P0 P1) := par (subst_proc_exp e x P0) ( subst_proc_exp e x P1);
@@ -286,21 +286,332 @@ subst_proc_exp e x inact := inact;
 
 
 Definition subst_nm (a x nm : atom) : atom :=
-if eq_atom x nm then a else nm.
+if x == nm then a else nm.
 
+(*parameterize this over some free variablesx*)
 
+(*added x in the catch case to see if forget proof becomes easier*)
 Equations subst_proc_nm (a x: atom)  (P : proc) : proc by wf (proc_size P)  :=
 subst_proc_nm a x (send nm e P0) := send (subst_nm a x nm) e (subst_proc_nm a x P0);
 subst_proc_nm a x (receive nm0 nm1 P0) := receive (subst_nm a x nm0) nm1 (subst_proc_nm a x P0);
 subst_proc_nm a x (throw nm0 nm1 P0) := throw (subst_nm a x nm0) (subst_nm a x nm1) (subst_proc_nm a x P0);
-subst_proc_nm a x (catch nm0 nm1 P0) := if eq_atom x nm1 then catch (subst_nm a x nm0) nm1 P0 
-                                                         else catch (subst_nm a x nm0) (fresh ([:: a]++ (fv P0))) (subst_proc_nm a x (swap nm1 (fresh ([:: a]++ (fv P0))) P0));
+subst_proc_nm a x (catch nm0 nm1 P0) := if x == nm1 then catch (subst_nm a x nm0) nm1 P0 
+                                                         else catch (subst_nm a x nm0) (set_fresh (add a (add x (fv_nm P0)))) (subst_proc_nm a x (swap nm1 (set_fresh (add a (add x (fv_nm P0)))) P0));
 subst_proc_nm a x (par P0 P1) := par (subst_proc_nm a x P0) ( subst_proc_nm a x P1);
 subst_proc_nm a x inact := inact;
-subst_proc_nm a x (nu_ch nm P0) := if eq_atom x nm then nu_ch nm P0 
-                                                   else nu_ch (fresh ([:: a] ++  (fv P0))) (subst_proc_nm a x (swap nm (fresh ([:: a] ++  (fv P0))) P0)).
+subst_proc_nm a x (nu_ch nm P0) := if x == nm then nu_ch nm P0 
+                                                   else nu_ch (set_fresh (add a (fv_nm P0))) (subst_proc_nm a x (swap nm (set_fresh (add a (fv_nm P0))) P0)).
 
-Reserved Notation "P --> Q" (at level 70).
+Notation "nm{ x ::= a } t" := (subst_nm a x t) (at level 70).
+
+Notation "p{ x ::= a } t" := (subst_proc_nm a x t) (at level 70).
+
+
+
+Ltac destruct_bool := match goal with
+                      | [  |- is_true (_ && _) -> _ ] =>  move=> /andP []
+                      | [  |- is_true (~~ (_ && _)) -> _ ] => rewrite negb_and; move=> /orP []
+
+                      end.
+
+
+Ltac reduce_in := rewrite /=  ?inE negb_or; destruct_bool.
+
+Lemma predC1_iff :  forall (a0 a1 : atom), (~~ predC1 a0 a1) <-> a0 == a1.
+Proof.
+move=> a0 a1. rewrite /predC1 /= Bool.negb_involutive. split; move/eqP=>->//=. 
+Qed.
+
+Lemma swap_aux_refl : forall a b, swap_aux a a b = b.
+Proof.
+move=> a b. rewrite /swap_aux. case : (eqVneq b a); done.
+Qed.
+
+Lemma swap_exp_refl : forall e a, swap_exp a a e = e.
+Proof.
+elim. 
+- move=> a. done. 
+- move=> a. done. 
+- move=> a a0. rewrite /swap_exp. rewrite swap_aux_refl. done. 
+Qed.
+
+Lemma swap_refl : forall p a, swap a a p = p.
+Proof.
+elim.
+- move=> a e p IH a0. rewrite /swap -/swap swap_aux_refl. rewrite swap_exp_refl. f_equal. done. 
+- move=> a a0 p IH a1.  rewrite /swap -/swap swap_aux_refl. rewrite swap_aux_refl. f_equal. done. 
+- move=> a a0 p IH a1.  rewrite /swap -/swap swap_aux_refl. rewrite swap_aux_refl. f_equal. done.  
+- move=> a a0 p IH a1.  rewrite /swap -/swap swap_aux_refl. rewrite swap_aux_refl. f_equal. done.  
+- move=> p IHp p0 IHp0 a.  rewrite /swap -/swap. rewrite IHp. rewrite IHp0. done. 
+- move => a. rewrite /=. done.
+- move=> a p IH a0.  rewrite /swap -/swap. rewrite IH. rewrite swap_aux_refl. done. 
+Qed.
+
+Ltac name_case a0 a1 := case : (eqVneq a0 a1).
+
+Lemma swap_inject : forall a a' bs bs', swap_aux bs bs' a = swap_aux bs bs' a' -> a  = a'.
+Proof.
+move => a a' bs bs'. rewrite /swap_aux.
+name_case a bs. 
+- move=>->. name_case a' bs.
+ + move=>->. done.
+ + name_case a' bs'. 
+  * move=>->. done.
+  * move=> /eqP H. move : (not_eq_sym H). done.
+- name_case a bs'.
+ + move=>->.  name_case a' bs.
+  * move=>->. done.
+  * name_case a' bs'. 
+   ** move=>->. done.
+   ** move=> H1 H2 H3 H4. move : H4 H1 H2 H3=>->. move => _. move/eqP. done.
+ + name_case a' bs.
+  * move=>->. move=> /eqP H _. done. 
+  * name_case a' bs'. 
+   ** move=>->. move => H1 H2 H3 H4. move : H4 H1 H2 H3=>->. move => _ _ /eqP. done.
+   ** done.
+Qed. 
+
+Definition swap_set bs bs' s := MapFunction.map (swap_aux bs bs') s. 
+
+
+Lemma in_swap_set : forall a bs bs' s, M.In a (swap_set bs bs' s) <-> exists a', M.In a' s /\ swap_aux bs bs' a' = a.
+Proof. 
+move => a bs bs' s. split;rewrite /swap_set; rewrite MapFunction.map_In //=; move=> x y-> //=.
+Qed.
+
+(*Some tactics*)
+Ltac contra := intros; subst; match goal with
+                    | [ H:  (is_true (negb (@eq_op nat_eqType ?a ?a)))  |- _ ] => by move : H=> /eqP
+
+                    | [ H: ?a <> ?a  |- _ ] => by move : H 
+
+                      end.
+
+Ltac ifN_tac :=  intro ; rewrite ifN_eq; [ | done ].
+Ltac ifNC_tac :=  intro ; rewrite ifN_eqC; [ | done ].
+
+Ltac get_eqs := try (match goal with
+                | [ H:  (is_true (_ (@eq_op nat_eqType _ _)))  |- _ ] => move : H
+                end).
+
+Ltac if_destruct := (try rewrite eq_refl) ; match goal with
+                    | [ |- context[if ?a == ?b then _ else _] ] => get_eqs; name_case a b; [move =>-> ; try rewrite eq_refl | try (ifN_tac + ifNC_tac) ]
+                    end ; try solve [contra | done ].
+
+Ltac if_destruct_r := repeat if_destruct.
+
+
+Lemma in_eqvt : forall a s bs bs', M.In a s <-> M.In (swap_aux bs bs' a) (swap_set bs bs' s).
+Proof. 
+move => a s bs bs'. split. 
+- rewrite in_swap_set. rewrite /swap_aux. if_destruct.  
+ * exists bs. rewrite eq_refl. split; done. 
+ * exists a. split. done. if_destruct. 
+- rewrite in_swap_set.  rewrite /swap_aux. 
+ * move => [] x [].  if_destruct.  
+  **  if_destruct. if_destruct_r. 
+  ** if_destruct_r. by move => + + + + <-.
+Qed.
+
+
+
+Lemma fv_nm_eqvt : forall P bs bs', M.Equal (swap_set bs bs' (fv_nm P)) (fv_nm (swap bs bs' P)).
+Proof. Admitted.
+
+
+Lemma in_fv_eqvt : forall P a bs bs', M.In a (fv_nm P) <-> M.In (swap_aux bs bs' a) (fv_nm (swap bs bs' P)).
+Proof.
+move => P a bs bs'. split. move/(in_eqvt _ _ bs bs'). rewrite fv_nm_eqvt. done.
+move => H.  rewrite (in_eqvt _ _ bs bs'). rewrite fv_nm_eqvt. done. 
+Qed.
+
+Lemma not_in_fv_equiv : forall P a bs bs', ~ M.In a (fv_nm P) <-> ~ M.In (swap_aux bs bs' a) (fv_nm (swap bs bs' P)).
+Proof.
+move => P a bs bs'. split. move => H2 H3. apply H2. rewrite in_eqvt.  rewrite fv_nm_eqvt. apply H3.   
+ move => H2 H3. apply H2. rewrite -in_fv_eqvt.  done. 
+Qed.
+
+Lemma swap_set_involutive : forall p bs bs', swap_set bs bs' (swap_set bs bs' p) = p.
+Proof. Admitted.
+
+
+Ltac forget_tac IH :=  
+  rewrite /fv_nm -/fv_nm; simp subst_proc_nm;
+  rewrite /subst_nm; if_destruct; (try fsetdec);
+  let H := fresh "H__in" in move=> H; rewrite /= ?eq_refl /=; apply IH; fsetdec.
+
+Lemma aeq_refl : forall P , P =A= P.
+Proof. 
+elim.
+- move => k e p H. by rewrite /= 2!eq_refl. 
+- move => k ep H. by rewrite /= 2!eq_refl. 
+- move => k e p H. by rewrite /= 2!eq_refl. 
+- move => k k' p H. by rewrite /= ?eq_refl. 
+- move => k k' p H. rewrite /= ?eq_refl. apply/andP. split; done.  
+- rewrite /=. done. 
+- move => k p H. by rewrite /= ?eq_refl. 
+Qed.
+
+
+
+(*Used by fresh Metalib tactic*)
+Ltac gather_atoms ::=
+  let A := gather_atoms_with (fun x : atoms => x) in
+  let B := gather_atoms_with (fun x : atom => M.singleton x) in
+  let C := gather_atoms_with (fun p : proc => fv_nm p) in
+
+  constr:(M.union A (M.union B C)).
+
+
+(*substitution lemmas*)
+Lemma subst_nm_refl : forall a b, nm{ a::=a} b = b.
+Proof. 
+move => a b. rewrite /subst_nm. if_destruct. 
+Qed. 
+
+Lemma subst_nm_refl2 : forall a b, nm{ a::=b} b = b.
+Proof. 
+move => a b. rewrite /subst_nm. name_case a b; done. 
+Qed. 
+
+Lemma subst_nm_match : forall a b, nm{ a::=b} a = b.
+Proof. 
+move => a b. rewrite /subst_nm. rewrite eq_refl. done. 
+Qed. 
+
+
+
+Check ind.
+(*This lemma is used in forget*)
+Lemma subst_fresh : forall p a b x x0, ~ M.In x (M.union (singleton a) (singleton b)) -> 
+                                  ~ M.In x0 (M.union (singleton a) (singleton b)) -> swap x x0 (p{ a ::= b } p) = (p{ a ::= b} swap x x0 p).
+Proof. Admitted.
+Lemma swap_aeq : forall p p' bs bs', p =A= p' -> swap bs bs' p =A= swap bs bs' p'.
+Proof. Admitted.
+
+Lemma swap_comm : forall p bs bs', swap bs bs' p = swap bs' bs p.
+Proof. Admitted.
+Require Import Wellfounded. 
+Check (well_founded_induction
+                     (wf_inverse_image _ nat _ (@proc_size)
+                        PeanoNat.Nat.lt_wf_0)).
+
+(*By size induction*)
+Lemma forget : forall  P a b, ~ M.In a (fv_nm P) ->  (p{a::= b} P) =A= P.
+Proof.
+move => + a b. induction P using (well_founded_induction
+                     (wf_inverse_image _ nat _ (@proc_size)
+                        PeanoNat.Nat.lt_wf_0)).
+destruct P. 
+-  forget_tac H.
+-  forget_tac H.
+-  rewrite /fv_nm -/fv_nm; simp subst_proc_nm. Print exp.
+  rewrite /subst_nm.  if_destruct_r; (try fsetdec).
+  move => neq H__in. rewrite /= ?eq_refl /=. apply H. fsetdec. fsetdec. 
+- rewrite /fv_nm -/fv_nm. 
+  simp  subst_proc_nm.  
+  if_destruct. 
+  * rewrite /subst_nm. if_destruct. 
+   ** fsetdec. 
+   ** by rewrite aeq_refl. 
+  * rewrite /subst_nm. if_destruct. 
+   ** fsetdec. 
+   **  move => H2 H3. rewrite /aeq -/aeq eq_refl /=. 
+       rewrite /set_fresh. destruct (atom_fresh ((add b (add a(fv_nm P))))). if_destruct. 
+    *** rewrite swap_refl. move => H5. apply H.  auto. move : H5=> /eqP => H4. have H__in: ~ M.In t0 ((singleton a)).  fsetdec. fsetdec. 
+    *** have: M.mem x (fv_nm P) = false. rewrite <- F.not_mem_iff. fsetdec. move=>->. move => H4 H5. rewrite swap_comm. 
+        apply H;auto. 
+     **** rewrite swap_size. auto.
+     **** rewrite -fv_nm_eqvt. rewrite (in_eqvt _ _ x t0). rewrite swap_set_involutive. rewrite /swap_aux. move : n.  if_destruct.
+      ***** fsetdec. 
+      ***** if_destruct. move : i0=> /eqP => H5. have : ~ M.In a (singleton t0) by fsetdec. fsetdec.
+Admitted.
+
+Lemma forget : forall  P a b, ~ M.In a (fv_nm P) ->  (p{a::= b} P) =A= P.
+Proof.
+move => + a b. apply  (@ind (M.union (M.singleton a) (M.singleton b)) (fun P => ~ M.In a (fv_nm P) -> (p{ a ::= b} P) =A= P)). 
+- admit. 
+- move => t e p IH. forget_tac IH. 
+- move => k x p H__nin IH. forget_tac IH.
+- move => k x p IH. 
+  rewrite /fv_nm -/fv_nm; simp subst_proc_nm. Print exp.
+  rewrite /subst_nm.  if_destruct_r; (try fsetdec).
+  move => neq H__in. rewrite /= ?eq_refl /=. apply IH. fsetdec. 
+- move => k x p _ IH. rewrite /fv_nm -/fv_nm. 
+  simp  subst_proc_nm.  
+  if_destruct. 
+  * rewrite /subst_nm. if_destruct. 
+   ** move => H2. fsetdec. 
+   ** rewrite aeq_refl. done. 
+  * rewrite /subst_nm. if_destruct. 
+   ** fsetdec. 
+   **  move => H2 H3. rewrite /aeq -/aeq eq_refl /=. 
+       rewrite /set_fresh. destruct (atom_fresh ((add b (add a(fv_nm p))))). name_case x0 x. 
+    *** move=>->.   rewrite swap_refl. apply IH.  move : H2=> /eqP => H4. have H__in: ~ M.In x ((singleton a)).  fsetdec. fsetdec. 
+    *** have: M.mem x0 (fv_nm p) = false. rewrite <- F.not_mem_iff. fsetdec. move=>->.
+  
+      apply singleton_iff.        Locate "!=". fsetdec.
+        if_destruct.
+    *** rewrite swap_refl. move => H5. apply IH. fsetdec. (*freshness of x is needed here*)
+    *** have: M.mem x0 (fv_nm p) = false. rewrite <- F.not_mem_iff. fsetdec. 
+        move =>->. move => H H2. rewrite swap_comm. rewrite -subst_fresh.  
+     **** apply swap_aeq. apply IH. fsetdec. 
+     **** fsetdec. 
+     **** fsetdec.      
+- admit. 
+- admit.
+-admit. 
+Admitted.
+
+Ltac forget_tac2 IH :=  
+  rewrite /fv_nm -/fv_nm; simp subst_proc_nm;
+  rewrite /subst_nm; if_destruct; (try fsetdec);
+  let H := fresh "H__in" in move=> H; rewrite /= ?eq_refl /=; move=>H2; apply H; fsetdec.
+
+Lemma forget2 : forall  P a b, ~ M.In a (fv_nm P) ->  (p{a::= b} P) =A= P.
+Proof.
+move => P a b. funelim  (p{ a ::= b} P).
+-  rewrite /fv_nm -/fv_nm; simp subst_proc_nm.
+  rewrite /subst_nm; if_destruct; (try fsetdec).
+  let H := fresh "H__in" in move=> H. rewrite /= ?eq_refl /=. move=>H2.  apply H. fsetdec.
+
+-   rewrite /fv_nm -/fv_nm; simp subst_proc_nm.
+  rewrite /subst_nm; if_destruct; (try fsetdec).
+  let H := fresh "H__in" in move=> H. rewrite /= ?eq_refl /=. move=>H2.  apply H. fsetdec.
+-
+  rewrite /fv_nm -/fv_nm; simp subst_proc_nm.
+  rewrite /subst_nm.  if_destruct_r; (try fsetdec).
+  move => neq H__in. rewrite /= ?eq_refl /=. move => H2. apply H. fsetdec. 
+- rewrite /fv_nm -/fv_nm. 
+  simp  subst_proc_nm.  
+  if_destruct. 
+  * rewrite /subst_nm. if_destruct. 
+   ** move => H2. fsetdec. 
+   ** rewrite aeq_refl. done. 
+  * rewrite /subst_nm. if_destruct. 
+   ** fsetdec. 
+   **  move => H2 H3 H4. rewrite /aeq -/aeq eq_refl /=. 
+    *** rewrite /set_fresh.  destruct (atom_fresh (add a (add x (fv_nm p2)))). 
+        if_destruct.  
+    *** rewrite swap_refl. move => H5. apply H. fsetdec. 
+    ***  rewrite /set_fresh. destruct (atom_fresh ((add b (add a(fv_nm p))))). have: M.mem x0 (fv_nm p) = false. rewrite <- F.not_mem_iff. fsetdec. move =>->. move => H H2.
+         rewrite -subst_fresh.  
+     **** f_equal. admit. 
+     **** fsetdec. 
+     **** fsetdec. 
+admit.     
+admit.
+admit.
+admit.
+
+
+
+
+
+(*The rest is unchanged, probably doesn't even run anymore*)
+
+ 
+ Reserved Notation "P --> Q" (at level 70).
 Inductive red : proc -> proc -> Prop :=
 | r_com k e nm P Q:
     (par (send k e P) (receive k nm Q)) --> (par P (subst_proc_exp e nm Q))
@@ -320,16 +631,9 @@ Inductive red : proc -> proc -> Prop :=
 
 where "P --> Q" := (red P Q).
 
-(*
-Ltac atom_destruct :=
-  repeat match goal with
-         | [ |- context[Atom.eq_dec ?e ?e0] ] 
-                => destruct (Atom.eq_dec e e0);try contradiction
-         | [ _ : context[Atom.eq_dec ?e ?e0]  |- _ ] 
-                => destruct (Atom.eq_dec e e0);try contradiction
-         end.
 
-Ltac atom_unf := rewrite /eqb ; atom_destruct.*)
+
+Definition k := fresh [::].
 
 Definition k0 := fresh [::].
 Definition k1 := fresh [::k0].
@@ -373,5 +677,5 @@ Proof.
 move => k0 k1 k2 k3 H H2. apply : r_cong. rewrite -congruent_iff. apply : c_refl. 2: { rewrite -congruent_iff. apply : c_inact. } apply : r_cong. rewrite -congruent_iff. apply c_refl. apply : r_pass. rewrite /=. rewrite inE.  
 rewrite unfold_in. destruct (eqVneq k1 k2). move : H=> /=. auto. rewrite /=. rewrite H2. rewrite /=. rewrite Bool.orb_false_r. auto.
 simp subst_proc_nm. rewrite /=. rewrite /subst_nm. do ? rewrite eq_atom_refl. rewrite /=//. 
-Qed.
+Qed
 
